Some modifications in the syntax, semantics and proof rules.
The syntax for allocation does not specify the length of the vector, just the vector. The semantics and proof rules are modifyed accordingly.

Q_State.thy
@@ -95,16 +95,6 @@ proof-
     by auto
 qed
 
-lemma ptensor_empty:"(ptensor_vec {} {} q1 q2) $ 0 = q1 $ 0 * q2 $ 0"
-proof-
-  interpret ps2:partial_state2 "[]" "{}" "{}" apply standard by auto
-  show ?thesis  unfolding ps2.ptensor_vec_def unfolding  
-    partial_state.tensor_vec_def  state_sig.d_def 
-   partial_state.encode1_def partial_state.dims1_def 
-    partial_state.encode2_def partial_state.dims2_def ps2.dims0_def ps2.vars0_def 
-    by auto
-qed
-
 lemma nths_set_gt_list_length:"nths l (- {0..<length l}) = []"
 proof -
   have "nths l (- {0..<length l}) ! 0 \<notin> set (nths l (- {0..<length l}))"
@@ -254,9 +244,9 @@ lemma idempoten_qstate:
 definition mapping::"'q set \<Rightarrow> 'q set \<Rightarrow> nat set \<times> nat set"
   where "mapping s1 s2 \<equiv>({},{})"
 
-typedef (overloaded) ('a::field)
+typedef (overloaded) ('a::comm_ring_1)
   QState = "{(s,v)| (s::nat set) (v::'a list).                                   
-              length v = (2^(card s)) \<and> finite s \<and> (length v = 1 \<longrightarrow> v\<noteq>[0])}"
+              length v = (2^(card s)) \<and> finite s}"
   morphisms uQState Abs_QState  
   by (rule exI[where x ="({},[1])"], auto)
 
@@ -272,31 +262,23 @@ lemma QState_rel1:"length(snd(uQState x)) = 2 ^ card (fst(uQState x))"
                   (((snd (uQState x)) ! 0) = 1)"
   by (transfer, auto) *)
 
-lemma QState_rel2:"length(snd(uQState x)) =  0 \<longrightarrow>
-                   (snd (uQState x)) \<noteq> [0]"
+lemma QState_rel3:"finite (fst (uQState (x::('a::comm_ring_1) QState )))"
   apply transfer by auto
 
 
-lemma QState_rel3:"finite (fst (uQState (x::('a::field) QState )))"
-  apply transfer by auto
+lift_definition QState_vars :: "('a::comm_ring_1) QState \<Rightarrow> nat set" is fst .
+lift_definition QState_list :: "('a::comm_ring_1) QState \<Rightarrow> 'a::comm_ring_1 list" is snd .
+lift_definition QState_vector::"('a::comm_ring_1) QState \<Rightarrow> 'a::comm_ring_1 vec" is "\<lambda>s. vec_of_list (snd s)" .
 
-
-
-lift_definition QState_vars :: "('a::field) QState \<Rightarrow> nat set" is fst .
-lift_definition QState_list :: "('a::field) QState \<Rightarrow> 'a list" is snd .
-lift_definition QState_vector::"('a::field) QState \<Rightarrow> 'a vec" is "\<lambda>s. vec_of_list (snd s)" .
-
-abbreviation QState_wf::"nat set \<times> 'a::field list \<Rightarrow> bool"
+abbreviation QState_wf::"nat set \<times> 'a::comm_ring_1 list \<Rightarrow> bool"
   where "QState_wf s \<equiv> 
-      length (snd s) = (2^(card (fst s))) \<and> 
-      finite (fst s) \<and> 
-      (length (snd s) = 1 \<longrightarrow> (snd s)\<noteq>[0])"
+      length (snd s) = (2^(card (fst s))) \<and> finite (fst s)"
 
-lift_definition QState :: "nat set \<times> 'a::field list \<Rightarrow> 'a QState" is  
+lift_definition QState :: "nat set \<times> 'a::comm_ring_1 list \<Rightarrow> 'a QState" is  
   "\<lambda>s. if QState_wf s then (fst s, snd s)
        else ({}, [1])"  by auto
 
-abbreviation QState_unfold ::"'a::field QState \<Rightarrow> nat set \<times> 'a::field list"
+abbreviation QState_unfold ::"'a::comm_ring_1 QState \<Rightarrow> nat set \<times> 'a::comm_ring_1 list"
   where "QState_unfold x \<equiv> (QState_vars x, QState_list x)"
 
 lemma QState_wf:"QState_wf (QState_unfold x)"
@@ -310,69 +292,20 @@ lemma QState_list_idem:"QState_wf (vs, v) \<Longrightarrow>
        QState_list (QState (vs, v)) = v"
   by (transfer, auto)
 
-lift_definition Conc :: " 'a QState \<Rightarrow> nat set \<times> 'a::field vec" is
+lift_definition Conc :: " 'a QState \<Rightarrow> nat set \<times> 'a::comm_ring_1 vec" is
   "\<lambda>s. (QState_vars s, QState_vector s)" .
 
-definition sca_mult_qstate::"'a::field \<Rightarrow> 'a QState \<Rightarrow> 'a QState"  (infixl "\<cdot>\<^sub>q" 70) 
+definition sca_mult_qstate::"'a::comm_ring_1 \<Rightarrow> 'a QState \<Rightarrow> 'a QState"  (infixl "\<cdot>\<^sub>q" 70) 
   where "sca_mult_qstate s qs \<equiv> QState(QState_vars qs, list_of_vec (s \<cdot>\<^sub>v (QState_vector qs)))"
 
-lemma sca_mult_qstate_wf:
-  assumes a0:"(s::'a::field) \<noteq> 0" 
-  shows "QState_wf (QState_vars qs, list_of_vec (s \<cdot>\<^sub>v (QState_vector qs)))"  
-proof-
-  have wf:"QState_wf (QState_unfold qs)"
-    using QState_wf by blast
-  
-  { assume "length (QState_list qs) = 1"    
-    then obtain v where v:"QState_list qs = [v] \<and> v \<noteq> 0"
-      using wf
-      by (metis One_nat_def Suc_length_conv length_0_conv snd_conv) 
-    then have "s * v \<noteq> 0" using a0 by auto
-    then have ?thesis using v
-    proof -
-      have "snd (uQState qs) = [v]"
-        by (metis (no_types) QState_list.rep_eq v)
-      then show ?thesis
-        by (metis (no_types) QState_rel1 QState_rel3 QState_vars.rep_eq 
-            QState_vector.rep_eq \<open>s * v \<noteq> 0\<close> dim_vec_of_list fst_conv 
-            index_smult_vec(1) index_smult_vec(2) neq0_conv snd_conv 
-            vec_index_vCons_0 vec_list vec_of_list_Cons zero_neq_one)
-    qed                                             
-  }
-  moreover { 
-    assume "length (QState_list qs) \<noteq> 1"
-    then have "dim_vec (vec_of_list (snd (uQState qs))) \<noteq> 1"
-        by (metis (full_types) QState_list.rep_eq  dim_vec_of_list)
-    then have ?thesis
-      by (simp add: QState_rel1 QState_rel3 QState_vars.rep_eq QState_vector.rep_eq)
-  }
-  ultimately show ?thesis by auto
-qed
-
-lemma sca_mult_qstate_vars:"(s::'a::field) \<noteq>0 \<Longrightarrow>QState_vars (s \<cdot>\<^sub>q qs) = QState_vars qs"
-  unfolding sca_mult_qstate_def using sca_mult_qstate_wf
-  using QState_var_idem by blast
-
-lemma sca_mult_qstate_quantum: 
-  "(s::'a::field) \<noteq>0 \<Longrightarrow> QState_vector (s \<cdot>\<^sub>q qs) = s \<cdot>\<^sub>v (QState_vector qs)"
-  unfolding sca_mult_qstate_def using sca_mult_qstate_wf[of s qs]  
-  apply transfer 
-  by (simp add: vec_list)
-
-lemma sca_mult_qstate_assoc: 
-  "a1 \<noteq> 0 \<Longrightarrow> a2\<noteq>0 \<Longrightarrow> (a1::'a::field)* a2 \<cdot>\<^sub>q qs = a1 \<cdot>\<^sub>q (a2 \<cdot>\<^sub>q qs)" 
-  by (metis (no_types) sca_mult_qstate_def 
-    sca_mult_qstate_quantum sca_mult_qstate_vars smult_smult_assoc)
-
-  
-definition empty_qstate::"'a::field QState"  ("|>") 
+definition empty_qstate::"'a::comm_ring_1 QState"  ("|>") 
   where "empty_qstate  \<equiv> QState({}, [1])"
 
 
 lemma uqstate_fst:"fst (uQState a) = QState_vars a" apply transfer' by auto
 lemma uqstate_snd:"snd (uQState a) = QState_list a" apply transfer' by auto
 
-lemma QState_rel3':"finite (QState_vars (x::('a::field) QState ))"
+lemma QState_rel3':"finite (QState_vars (x::('a::comm_ring_1) QState ))"
   by (transfer, auto)
 
 lemma QState_rel1':"length(QState_list x) = 2 ^ card (QState_vars x)"
@@ -435,31 +368,21 @@ lemma fst_uQState_not_empty_wf_uQState:"fst (uQState a) \<noteq> {} \<Longrighta
 lemma QState_refl:"QState (QState_vars a, QState_list a) = a"
   by (transfer, auto)
 
-lemma QState_var_qstate:"QState_vars (QState (QState_vars a, QState_list a)) = QState_vars a"
+lemma "QState_vars (QState (QState_vars a, QState_list a)) = QState_vars a"
   by (simp add:  QState_refl)
 
-lemma QState_list_qstate:"QState_list (QState (QState_vars a, QState_list a)) = QState_list a"
+lemma "QState_list (QState (QState_vars a, QState_list a)) = QState_list a"
   by (simp add:  QState_refl)
 
-lemma QState_list_empty:"QState_vars Q = {} \<Longrightarrow> \<exists>v. QState_list Q = [v]"
-  by (metis One_nat_def QState_rel1' Suc_length_conv card_empty 
-      list_exhaust_size_eq0 power.simps(1))
-  
-lemma QState_list_inv: assumes a0:"QState_vars Q = {}"
-  shows "inverse(QState_list Q ! 0) \<cdot>\<^sub>q Q = |>"
-  unfolding empty_qstate_def sca_mult_qstate_def using a0 apply transfer' 
-  apply auto
-  by (simp add: list_of_vec_map vec_of_list_index)
-  
 
-definition plus_QState_vector::"('a::field) QState \<Rightarrow> 'a QState \<Rightarrow>nat set \<times> 'a list"
+definition plus_QState_vector::"('a::comm_ring_1) QState \<Rightarrow> 'a QState \<Rightarrow>nat set \<times> 'a list"
   where "plus_QState_vector q1 q2 \<equiv> 
      let d1 = QState_vars q1; 
          d2 = QState_vars q2; 
          l1 = QState_vector q1; l2 = QState_vector q2 in
           (d1 \<union> d2, list_of_vec(partial_state2.ptensor_vec d1 d2 l1 l2))"
 
-definition vector_element_12::"('a::field) QState \<Rightarrow> nat set \<Rightarrow> nat \<times> nat \<Rightarrow> 'a"
+definition vector_element_12::"('a::comm_ring_1) QState \<Rightarrow> nat set \<Rightarrow> nat \<times> nat \<Rightarrow> 'a"
   where "vector_element_12 v d1 p \<equiv> 
          let d = QState_vars v; 
          d2 = d - d1; 
@@ -500,13 +423,13 @@ proof-
      using  v1  apply transfer' by (auto simp add: list_vec)          
 qed
 
-definition plus_QState:: "('a::field) QState \<Rightarrow> 'a QState \<Rightarrow> 'a QState"
+definition plus_QState:: "('a::comm_ring_1) QState \<Rightarrow> 'a QState \<Rightarrow> 'a QState"
   where "plus_QState q1 q2 \<equiv> 
     let d1 = (QState_vars q1); d2 = (QState_vars q2) in
       if (d1 \<inter> d2 \<noteq> {}) then QState ({},[1])
       else QState (plus_QState_vector q1 q2)"
 
-definition disj_QState::"('a::field) QState \<Rightarrow> 'a QState \<Rightarrow> bool"
+definition disj_QState::"('a::comm_ring_1) QState \<Rightarrow> 'a QState \<Rightarrow> bool"
   where "disj_QState q1 q2 \<equiv> QState_vars q1 \<inter> QState_vars q2 = {}"
 
 \<comment>\<open>Lemmas on plus_QState_vector\<close>
@@ -589,27 +512,6 @@ lemma plus_QState_vector_wf: assumes a0: "QState_vars q1 \<inter> QState_vars q2
   apply clarsimp  apply (frule plus_QState_vector_wf')  
   by force+
 
-lemma plus_QState_vector_wf_empty:
-  assumes a0:"QState_vars q1 \<inter> QState_vars q2 = {}" and
-          a1:"fst (plus_QState_vector q1 q2) = {}"
-        shows "snd (plus_QState_vector q1 q2) \<noteq> [0]"
-proof-
-  have "QState_vars q1 = {}" and "QState_vars q2 = {}"
-    using a1 unfolding plus_QState_vector_def Let_def by auto  
-  moreover have "QState_vector q1 $ 0 \<noteq> 0" and "QState_vector q2 $ 0 \<noteq> 0"
-    using calculation apply auto apply transfer
-     apply (metis One_nat_def Suc_length_conv card_empty fstI 
-              list_exhaust_size_eq0 nth_Cons_0 power_0 sndI vec_of_list_index)
-    apply transfer
-    by (metis One_nat_def Suc_length_conv card_empty fstI 
-              list_exhaust_size_eq0 nth_Cons_0 power_0 sndI vec_of_list_index)
-  ultimately have "(ptensor_vec (QState_vars q1) (QState_vars q2) (QState_vector q1)
-            (QState_vector q2)) $ 0 \<noteq> 0" 
-    using ptensor_empty[of "QState_vector q1" "QState_vector q2"] by simp
-  then show ?thesis unfolding plus_QState_vector_def Let_def
-    by (metis nth_Cons_0 snd_conv vec_list vec_of_list_index)                                                     
-qed
-
 (* lemma plus_QState_vector_empty_vars_one_wf:
   assumes a0:"fst (plus_QState_vector q1 q2) = {} " 
   shows "snd (plus_QState_vector q1 q2) = [1]"
@@ -632,8 +534,8 @@ lemma QState_vars_Plus:"(QState_vars q1 \<inter> QState_vars q2 \<noteq> {} \<lo
            QState_vars (plus_QState q1 q2) = fst (plus_QState_vector q1 q2))"  
     apply (auto simp add: plus_QState_def ) apply transfer
     apply simp 
-   apply transfer' using plus_QState_vector_set_wf plus_QState_vector_wf
-  apply (smt QState_id_fst_empty empty_iff prod.collapse snd_uQState_empty)
+   apply transfer' using plus_QState_vector_set_wf plus_QState_vector_wf  
+   apply (smt fst_conv)
    apply transfer' using plus_QState_vector_set_wf plus_QState_vector_wf
   by fastforce
 
@@ -645,10 +547,8 @@ lemma QState_list_Plus:"(QState_vars q1 \<inter> QState_vars q2 \<noteq> {} \<lo
     apply auto
   apply transfer 
   apply auto 
-  using plus_QState_vector_set_wf
-  apply blast
-  using plus_QState_vector_wf apply blast
-  using plus_QState_vector_wf_empty by auto
+  using plus_QState_vector_set_wf     
+  by (auto simp add: plus_QState_vector_wf) 
 
 lemma neutral_vector_wf:"length [1] = (2^(card {}))" by auto
 
@@ -687,6 +587,8 @@ proof-
   }
   ultimately show ?thesis by auto 
 qed
+typedef natsub = "{x. x<(10::nat)}"
+  by (meson mem_Collect_eq zero_less_numeral)
   
 
 lemma plus_comm:"disj_QState x y \<Longrightarrow> plus_QState x y = plus_QState y x"
@@ -736,6 +638,8 @@ lemma nths_eq:"v = {0..<card v} \<Longrightarrow>
   by (smt Collect_cong add_cancel_left_right append_Nil2 atLeast0LessThan le_add_same_cancel1 
           length_append length_nths length_replicate lessThan_iff less_le_trans 
           list_exhaust_size_eq0 nths_append zero_le)
+
+
 
 lemma QState_list_assoc:
    assumes a0:"QState_vars x  \<inter> QState_vars y = {}" and
@@ -811,7 +715,7 @@ proof-
 qed
 
 
-instantiation QState :: (field) sep_algebra
+instantiation QState :: (comm_ring_1) sep_algebra
 begin
 definition zero_QState: "0 \<equiv> QState ({},[1])"
 definition plus_QState: "s1 + s2 \<equiv> plus_QState s1 s2" 
@@ -829,73 +733,6 @@ instance
   done
 end 
 
-lemma scalar_mult_QState_plus_l:
-  assumes a0: "(a::'a::field) \<noteq> 0" and 
-          a1:"Q' ## Q''"
-        shows "a  \<cdot>\<^sub>q (Q' + Q'') = (a  \<cdot>\<^sub>q Q' + Q'')"
-proof-
-  let ?q'vs = "QState_vars Q'" and ?q''vs = "QState_vars Q''" and
-      ?q'v = "QState_vector Q'" and ?q''v = "QState_vector Q''"
-  note a1 = a1[simplified disj_QState_def sep_disj_QState]
-  have "QState_vars (a  \<cdot>\<^sub>q (Q' + Q'')) = QState_vars (Q' + Q'')"
-    by (simp add: a0 sca_mult_qstate_vars)
-  moreover have "QState_vector (a  \<cdot>\<^sub>q (Q' + Q'')) = a \<cdot>\<^sub>v (QState_vector (Q' + Q''))"
-    by (meson a0 sca_mult_qstate_quantum)  
-  moreover have "a \<cdot>\<^sub>v (QState_vector (Q' + Q'')) = 
-                 a \<cdot>\<^sub>v (ptensor_vec ?q'vs ?q''vs ?q'v ?q''v)"
-    using a1 
-    unfolding plus_QState_vector_def disj_QState_def sep_disj_QState plus_QState plus_QState_def Let_def sca_mult_qstate_def
-    apply auto    
-    by (metis QState_list_Plus QState_vector.rep_eq plus_QState_def plus_QState_vector_def plus_QState_vector_vector uqstate_snd vec_list)
-  then have " a \<cdot>\<^sub>v (QState_vector (Q' + Q'')) = 
-                  (ptensor_vec ?q'vs ?q''vs (a \<cdot>\<^sub>v ?q'v) ?q''v)" 
-    by (simp add:pscalar_ptensor_1[OF a1] QState_rel1' QState_rel3' QState_vector.rep_eq uqstate_snd)   
-  moreover have  "QState_vars (a  \<cdot>\<^sub>q Q' + Q'') = QState_vars (Q' + Q'')"
-    by (metis (no_types, lifting) QState_vars_Plus a0 plus_QState plus_QState_vector_vars sca_mult_qstate_vars)
-  moreover have "QState_vector (a  \<cdot>\<^sub>q Q' + Q'') =  
-                 ptensor_vec ?q'vs ?q''vs (a  \<cdot>\<^sub>v ?q'v) ?q''v"
-    using calculation(3)
-    by (smt QState_vars_Plus a0 a1  plus_QState plus_QState_def 
-            plus_QState_vector_def plus_QState_vector_vars 
-            sca_mult_qstate_def sca_mult_qstate_quantum sca_mult_qstate_vars)
-  ultimately show ?thesis
-    by (metis QState_refl QState_vector.rep_eq list_vec uqstate_snd)
-qed
-
-lemma scalar_mult_QState_plus_r: 
-  assumes a0: "(a::'a::field) \<noteq> 0" and 
-          a1:"Q' ## Q''" 
-  shows "a  \<cdot>\<^sub>q (Q' + Q'') = ( Q' + a  \<cdot>\<^sub>q Q'')"
-proof-
-let ?q'vs = "QState_vars Q'" and ?q''vs = "QState_vars Q''" and
-      ?q'v = "QState_vector Q'" and ?q''v = "QState_vector Q''"
-  note a1 = a1[simplified disj_QState_def sep_disj_QState]
-  have "QState_vars (a  \<cdot>\<^sub>q (Q' + Q'')) = QState_vars (Q' + Q'')"
-    by (simp add: a0 sca_mult_qstate_vars)
-  moreover have "QState_vector (a  \<cdot>\<^sub>q (Q' + Q'')) = a \<cdot>\<^sub>v (QState_vector (Q' + Q''))"
-    by (meson a0 sca_mult_qstate_quantum)  
-  moreover have "a \<cdot>\<^sub>v (QState_vector (Q' + Q'')) = 
-                 a \<cdot>\<^sub>v (ptensor_vec ?q'vs ?q''vs ?q'v ?q''v)"
-    using a1 
-    unfolding plus_QState_vector_def disj_QState_def sep_disj_QState plus_QState plus_QState_def Let_def sca_mult_qstate_def
-    apply auto    
-    by (metis QState_list_Plus QState_vector.rep_eq plus_QState_def plus_QState_vector_def plus_QState_vector_vector uqstate_snd vec_list)
-  then have " a \<cdot>\<^sub>v (QState_vector (Q' + Q'')) = 
-                  (ptensor_vec ?q'vs ?q''vs ?q'v (a \<cdot>\<^sub>v ?q''v))" 
-    by (simp add:pscalar_ptensor_2[OF a1] QState_rel1' QState_rel3' QState_vector.rep_eq uqstate_snd)   
-  moreover have  "QState_vars (Q' + a  \<cdot>\<^sub>q Q'') = QState_vars (Q' + Q'')"
-    by (metis (no_types, lifting) QState_vars_Plus a0 plus_QState plus_QState_vector_vars sca_mult_qstate_vars)
-  moreover have "QState_vector (Q' + a  \<cdot>\<^sub>q Q'') =  
-                 ptensor_vec ?q'vs ?q''vs ?q'v (a  \<cdot>\<^sub>v ?q''v)"
-    using calculation(3) 
-    by (smt QState_vars_Plus a0 a1  plus_QState plus_QState_def 
-            plus_QState_vector_def plus_QState_vector_vars 
-            sca_mult_qstate_def sca_mult_qstate_quantum sca_mult_qstate_vars)
-  ultimately show ?thesis
-    by (metis QState_refl QState_vector.rep_eq list_vec uqstate_snd)
-qed
-
-
 type_synonym q_vars = "(nat \<Rightarrow>nat set)"
 type_synonym  'a qstate = "q_vars \<times> 'a QState"
 
@@ -906,38 +743,37 @@ definition ket_dim ::"q_vars \<Rightarrow> nat"
   where "ket_dim q_vars \<equiv>  card (Q_domain q_vars)"
 
 \<comment>\<open>\<close>
-abbreviation QStateM_wf::"q_vars \<times> ('a::field QState) \<Rightarrow> bool"
+abbreviation QStateM_wf::"q_vars \<times> ('a::comm_ring_1 QState) \<Rightarrow> bool"
   where "QStateM_wf s \<equiv> 
         Q_domain (fst s) = QState_vars (snd s) \<and>
         (\<forall>x y. x\<noteq>y \<and> x\<in> domain (fst s) \<and> y \<in> domain (fst s) \<longrightarrow> (fst s) x \<inter> (fst s) y = {})"
 
-typedef (overloaded) ('a::field)
+typedef (overloaded) ('a::comm_ring_1)
   QStateM = "{(m,q)| (m::q_vars) (q:: 'a QState). QStateM_wf (m,q)}"
   morphisms uQStateM Abs_QStateM              
   unfolding Q_domain_def  apply auto apply transfer
   apply (rule exI[where x ="\<lambda>x. {}"], auto)
-  by (rule exI[where x ="[1]"], auto)
+  by (metis length_Cons list.size(3) nth_Cons_0)
 
 setup_lifting type_definition_QStateM
 
-lift_definition QStateM_map :: "('a::field) QStateM \<Rightarrow> q_vars" is fst .
+lift_definition QStateM_map :: "('a::comm_ring_1) QStateM \<Rightarrow> q_vars" is fst .
 
 abbreviation empty_map::"q_vars" ("{}\<^sub>q")
   where "empty_map \<equiv> (\<lambda>n. {})"
 
-definition qstate :: "('a::field) QStateM \<Rightarrow> 'a QState" 
+definition qstate :: "('a::comm_ring_1) QStateM \<Rightarrow> 'a::comm_ring_1 QState" 
   where "qstate s \<equiv> snd (uQStateM s)"
 
-lift_definition QStateM_vars::"('a::field) QStateM \<Rightarrow> nat set" is "(\<lambda>s. QState_vars (snd s))" .
-lift_definition QStateM_list::"('a::field) QStateM \<Rightarrow> 'a list" is "(\<lambda>s. QState_list (snd s))" .
-lift_definition QStateM_vector::"('a::field) QStateM \<Rightarrow> 'a vec" is "(\<lambda>s. QState_vector (snd s))" .
+lift_definition QStateM_vars::"('a::comm_ring_1) QStateM \<Rightarrow> nat set" is "(\<lambda>s. QState_vars (snd s))" .
+lift_definition QStateM_list::"('a::comm_ring_1) QStateM \<Rightarrow> 'a list" is "(\<lambda>s. QState_list (snd s))" .
+lift_definition QStateM_vector::"('a::comm_ring_1) QStateM \<Rightarrow> 'a vec" is "(\<lambda>s. QState_vector (snd s))" .
 
-lift_definition QStateM ::"q_vars \<times> ('a::field QState) \<Rightarrow> 'a QStateM" is
+lift_definition QStateM ::"q_vars \<times> ('a::comm_ring_1 QState) \<Rightarrow> 'a QStateM" is
 "\<lambda>s. if QStateM_wf s then (fst s, snd s) else (\<lambda>s. {}, QState ({},[1]))"
   unfolding Q_domain_def by (auto simp add:  QState_vars_empty)
 
-
-abbreviation QStateM_unfold::"('a::field) QStateM \<Rightarrow> (q_vars \<times> 'a QState)"
+abbreviation QStateM_unfold::"('a::comm_ring_1) QStateM \<Rightarrow> (q_vars \<times> 'a::comm_ring_1 QState)"
   where "QStateM_unfold q \<equiv> (QStateM_map q, qstate q)"
 
 lemma eq_QStateM_vars:"QState_vars (snd (QStateM_unfold q)) = QStateM_vars q"
@@ -1015,57 +851,6 @@ lemma a1:"\<Union> (range (0::nat \<Rightarrow> nat set)) = none"
 lemma a2:"QState_vars 0 = 0"
   by (simp add: QState_vars_empty zero_QState zero_set_def)
 
-definition sca_mult_qstatem::"'a::field \<Rightarrow> 'a QStateM \<Rightarrow> 'a QStateM"  (infixl "\<cdot>\<^sub>Q" 70)
-  where "sca_mult_qstatem s qs \<equiv> QStateM(QStateM_map qs, s \<cdot>\<^sub>q (qstate qs))"
-
-lemma sca_mult_qstatem_wf:
-  assumes a0:"(s::'a::field) \<noteq> 0" shows "QStateM_wf (QStateM_map qs, s \<cdot>\<^sub>q (qstate qs))"
-proof-
-  have "QStateM_wf (QStateM_unfold qs)"
-    using QStateM_wf by blast
-  thus ?thesis using sca_mult_qstate_vars a0
-    by (simp add: sca_mult_qstate_vars[OF a0])
-qed
-
-lemma sca_mult_qstatem_var_map:
-  "(s::'a::field) \<noteq> 0 \<Longrightarrow> QStateM_map (s \<cdot>\<^sub>Q qs) = QStateM_map qs"
-  unfolding sca_mult_qstatem_def using sca_mult_qstatem_wf[of s qs]
-  by (auto simp add: QStateM_wf_map)
-
-lemma sca_mult_qstatem_var_qstate:
-  "(s::'a::field) \<noteq> 0 \<Longrightarrow> qstate (s \<cdot>\<^sub>Q qs) = s \<cdot>\<^sub>q qstate qs"
-  unfolding sca_mult_qstatem_def using sca_mult_qstatem_wf[of s qs]
-  by (auto simp add: QStateM_wf_qstate)
-
-lemma QStateM_list_inv: assumes a0:"Q_domain (QStateM_map \<Q>) = {}"
-  shows "inverse(QStateM_list \<Q> ! 0) \<cdot>\<^sub>Q \<Q> = QStateM (\<lambda>x. {}, 0)"
-proof-
-  have "QStateM_map \<Q> = {}\<^sub>q" using a0 unfolding Q_domain_def by auto       
-  moreover have "QStateM_list \<Q> = QState_list (qstate \<Q>)"
-    unfolding qstate_def apply transfer by auto
-  moreover have  "inverse(QState_list (qstate \<Q>) ! 0) \<cdot>\<^sub>q (qstate \<Q>) = 0"  
-    unfolding zero_QState empty_qstate_def
-    using QStateM_rel1 QState_list_inv assms empty_qstate_def by fastforce
-  ultimately show ?thesis unfolding sca_mult_qstatem_def 
-    by auto
-qed
-
-lemma sca_mult_qstatem_assoc: 
-  "a1 \<noteq> 0 \<Longrightarrow> a2\<noteq>0 \<Longrightarrow> (a1::'a::field)* a2 \<cdot>\<^sub>Q Q = a1 \<cdot>\<^sub>Q (a2 \<cdot>\<^sub>Q Q)"
-  by (metis (no_types) sca_mult_qstate_assoc sca_mult_qstatem_def sca_mult_qstatem_var_map sca_mult_qstatem_var_qstate)
-
-
-lemma QStateM_empty_not_zero: assumes a0:"Q_domain (QStateM_map \<Q>) = {}"
-  shows "(QStateM_list \<Q> ! 0) \<noteq> 0"
-proof-
-  have "QStateM_map \<Q> = {}\<^sub>q" using a0 unfolding Q_domain_def by auto       
-  then have "QStateM_list \<Q> = QState_list (qstate \<Q>)"
-    unfolding qstate_def apply transfer by auto  
-  then show ?thesis apply auto unfolding qstate_def
-    by (metis One_nat_def QStateM_rel1 QState_list_empty QState_wf assms 
-        length_Cons list.size(3) nth_Cons_0 qstate_def snd_conv)
-qed
-
 lemma disjoint_x_y_wf1_x_plus_y:
        assumes a0:"QStateM_map x ## QStateM_map y "  and 
               a1:"qstate x ## qstate y"
@@ -1131,7 +916,7 @@ lemma plus_wf: assumes a0:"QStateM_map x ## QStateM_map y "  and
   apply transfer' apply auto 
   sorry *)
 
-instantiation QStateM :: (field) sep_algebra
+instantiation QStateM :: (comm_ring_1) sep_algebra
 begin
 definition zero_QStateM: "0 \<equiv> QStateM (0, 0)"
 definition plus_QStateM: "s1 + s2 \<equiv> QStateM (QStateM_map s1 + QStateM_map s2, qstate s1 + qstate s2)" 
@@ -1166,20 +951,7 @@ instance
   by (smt sep_disj_QStateM Qstate_mapf Qstate_vector 
           disjoint_x_y_wf1_x_plus_y fst_conv plus_QStateM plus_wf 
            sep_disj_add sep_disj_addD)  
-end 
+end
 
-lemma scalar_mult_QStateM_plus_l:
-  "(a::'a::field) \<noteq> 0 \<Longrightarrow> \<Q>' ## \<Q>'' \<Longrightarrow> a  \<cdot>\<^sub>Q (\<Q>' + \<Q>'') = (a  \<cdot>\<^sub>Q \<Q>' + \<Q>'')"
-  unfolding sca_mult_qstatem_def plus_QStateM sep_disj_QStateM
-  by (smt QStateM_wf_map QStateM_wf_qstate plus_wf sca_mult_qstatem_wf 
-          scalar_mult_QState_plus_l)
-  
 
-lemma scalar_mult_QStateM_plus_r:
-  assumes a0:"(a::'a::field) \<noteq> 0" and a1:"\<Q>' ## \<Q>''" 
-  shows "a  \<cdot>\<^sub>Q (\<Q>' + \<Q>'') = ( \<Q>' + a  \<cdot>\<^sub>Q \<Q>'')"
-  by (smt a0 assms(2) plus_QStateM sca_mult_qstatem_def sca_mult_qstatem_var_map 
-       sca_mult_qstatem_var_qstate scalar_mult_QStateM_plus_l 
-         scalar_mult_QState_plus_l scalar_mult_QState_plus_r sep_disj_QStateM)
- 
 end
